Log rep with header in a single block, post-conditions proofs for append and truncate

src/ChecksumLog.v
@@ -11,287 +11,132 @@ Require Import Cache.
 Require Import Omega.
 Require Import GenSep.
 Require Import PredCrash.
+Require Import Rec.
 
+Import ListNotations.
 Set Implicit Arguments.
 
-Definition PreviousLength : addr := $0.
-Definition CurrentLength : addr := $1.
-Definition Checksum : addr := $2.
-Definition DataStart : addr := $3.
+Definition header_type : Rec.type := Rec.RecF ([
+    ("previous_length",  Rec.WordF addrlen);
+    ("current_length",  Rec.WordF addrlen);
+    ("checksum",   Rec.WordF hashlen);
+    ("padding", Rec.WordF (valulen - hashlen - addrlen - addrlen))
+  ]).
+Definition header := Rec.data header_type.
+Definition make_header : header := (@Rec.of_word header_type $0)
+                                :=> "checksum" := default_hash.
+
+Theorem header_len :
+  valulen = Rec.len header_type.
+Proof.
+  simpl. rewrite valulen_is. compute. auto.
+Qed.
+
+Definition header_to_valu (h : header) : valu.
+  rewrite header_len.
+  exact (Rec.to_word h).
+Defined.
+
+Definition valu_to_header (v : valu) : header.
+  rewrite header_len in *.
+  exact (Rec.of_word v).
+Defined.
+
 Parameter maxlen : addr.
+Definition Header : addr := $0.
+Definition DataStart : addr := $1.
 
 Definition list_prefix A (p l : list A) :=
   firstn (length p) l = p.
 
-Definition log_rep_prefix h len vl vdisk hm :=
-  hash_list_rep (rev vl) h hm /\
-  list_prefix vl vdisk /\
-  length vl = len.
-
-(* EVentually len' can live in memory *)
-Definition log_rep vl vl' vdisk hm :
+(** Log_rep:
+  - The current list of values in the log is a prefix of the disk.
+  - The checksum and current_length in the header matches the current
+    list of values (previous_length can be anything)
+  Eventually current_length can live in memory **)
+Definition log_rep previous_length vl vdisk hm :
   @pred addr (@weq addrlen) valuset :=
-  (exists h h' len len',
-    [[ log_rep_prefix h len vl vl' hm ]] *
-    [[ log_rep_prefix h' len' vl' vdisk hm ]] *
+  (exists h current_length,
+    let header := make_header
+      :=> "previous_length" := ($ previous_length)
+      :=> "current_length"  := ($ current_length)
+      :=> "checksum"        := h
+    in
+    [[ hash_list_rep (rev vl) h hm ]] *
+    [[ length vl = current_length ]] *
+    [[ list_prefix vl vdisk ]] *
     [[ length vdisk = # (maxlen) ]] *
-    PreviousLength |-> (addr2valu $ (len), nil) *
-    CurrentLength |-> (addr2valu $ (len'), nil) *
-    Checksum |-> (hash_to_valu h', nil) *
+    Header |-> (header_to_valu header, nil) *
     array DataStart (combine vdisk (repeat nil # (maxlen))) $1)%pred.
-
-Definition crep vl vl' vl'' vdisk hm :
-  @pred addr (@weq addrlen) valuset :=
-  (exists h h' h'' len len' len'' unsynced_data,
-    [[ log_rep_prefix h len vl vl' hm ]] *
-    [[ log_rep_prefix h' len' vl' vl'' hm ]] *
-    [[ log_rep_prefix h'' len'' vl'' vdisk hm ]] *
-    (PreviousLength |-> (addr2valu $ (len), nil) \/
-      PreviousLength |-> (addr2valu $ (len'), addr2valu $ (len) :: nil)) *
-    (CurrentLength |-> (addr2valu $ (len'), nil) \/
-      CurrentLength |-> (addr2valu $ (len''), addr2valu $ (len') :: nil)) *
-    (Checksum |-> (hash_to_valu h', nil) \/
-      Checksum |-> (hash_to_valu h'', hash_to_valu h' :: nil)) *
-    (array DataStart (combine vdisk
-        (upd (repeat nil # (maxlen)) $ ( len') (unsynced_data :: nil))) $1)
-  )%pred.
-
-(** What the rep *should* be after crash.
-- PreviousHash points to a synced hash value that matches a
-  prefix of the disk.
-- NextHash points to a synced hash value. If this hash matches
-  a prefix of the disk, then PreviousHash's matched disk prefix
-  is also a prefix of NextHash's disk prefix.
-- DataStart points to a synced array.
-
-Definition log_rep_part vl hm vdisk :
-  @pred addr (@weq addrlen) valuset :=
-  (exists h h',
-    [[ log_rep_prefix h vl vdisk # (maxlen) hm ]] *
-    [[ (exists vl', log_rep_prefix h' vl' vdisk # (maxlen) hm
-        -> list_prefix vl vl') ]] *
-    PreviousHash |-> (hash_to_valu h, nil) *
-    NextHash |-> (hash_to_valu h', nil) *
-    array DataStart (combine vdisk (repeat nil # (maxlen))) $1
-  )%pred.**)
 
 Definition log_rep' vl vl' hm cs d : pred :=
   BUFCACHE.rep cs d *
   [[ (exists vdisk, log_rep vl vl' vdisk hm)%pred d ]].
 
-Definition possible_crash_list (l: list valuset) (l': list valu) :=
-  length l = length l' /\ forall i, i < length l -> In (selN l' i $0) (valuset_list (selN l i ($0, nil))).
-
-Lemma crash_xform_array: forall l start stride,
-  crash_xform (array start l stride) =p=>
-    exists l', [[ possible_crash_list l l' ]] * array start (List.combine l' (repeat nil (length l'))) stride.
-Proof.
-Admitted.
-
-Lemma crash_invariant_synced_array: forall l start stride,
-  crash_xform (array start (List.combine l (repeat nil (length l))) stride) =p=>
-  array start (List.combine l (repeat nil (length l))) stride.
-Proof.
-Admitted.
-
-Lemma crash_xform_helper : forall vdisk log_pointer unsynced_data,
-  crash_xform (array DataStart (combine vdisk
-        (upd (repeat nil (length vdisk)) log_pointer (unsynced_data :: nil))) $1) =p=>
-    array DataStart (combine vdisk (repeat nil (length vdisk))) $1 \/
-    array DataStart (combine (upd vdisk log_pointer unsynced_data) (repeat nil (length vdisk))) $1.
-Proof.
-Admitted.
-
-Definition read T i (log_pointer : addr) cs rx : prog T :=
-  let^ (cs, v) <- BUFCACHE.read_array DataStart i $1 cs;
-  rx ^(cs, log_pointer, v).
-
 Definition append T v cs rx : prog T :=
-  let^ (cs, log_pointer) <- BUFCACHE.read CurrentLength cs;
-  let^ (cs, h) <- BUFCACHE.read Checksum cs;
-  h <- Hash (Word.combine v (valu_to_hash h));
-  cs <- BUFCACHE.write_array DataStart (valu2addr log_pointer) $1 v cs;
-  cs <- BUFCACHE.write PreviousLength log_pointer cs;
-  cs <- BUFCACHE.write CurrentLength (addr2valu (valu2addr log_pointer ^+ $1)) cs;
-  cs <- BUFCACHE.write Checksum (hash_to_valu h) cs;
-  cs <- BUFCACHE.sync_array DataStart (valu2addr log_pointer) $1 cs;
-  cs <- BUFCACHE.sync PreviousLength cs;
-  cs <- BUFCACHE.sync CurrentLength cs;
-  cs <- BUFCACHE.sync Checksum cs;
+  let^ (cs, header_valu) <- BUFCACHE.read Header cs;
+  let header := valu_to_header header_valu in
+  let log_pointer := header :-> "current_length" in
+  checksum <- Hash (Word.combine v (header :-> "checksum"));
+  cs <- BUFCACHE.write_array DataStart log_pointer $1 v cs;
+  cs <- BUFCACHE.write Header (header_to_valu (
+          make_header
+            :=> "previous_length" := log_pointer
+            :=> "current_length" := log_pointer ^+ $1
+            :=> "checksum" := checksum
+          )) cs;
+  cs <- BUFCACHE.sync_array DataStart log_pointer $1 cs;
+  cs <- BUFCACHE.sync Header cs;
   rx cs.
 
 Definition truncate T cs rx : prog T :=
-  h <- Hash default_valu;
-  cs <- BUFCACHE.write PreviousLength $0 cs;
-  cs <- BUFCACHE.write CurrentLength $0 cs;
-  cs <- BUFCACHE.write Checksum (hash_to_valu h) cs;
-  cs <- BUFCACHE.sync PreviousLength cs;
-  cs <- BUFCACHE.sync CurrentLength cs;
-  cs <- BUFCACHE.sync Checksum cs;
+  hash0 <- Hash default_valu;
+  cs <- BUFCACHE.write Header (header_to_valu (
+          make_header
+            :=> "previous_length" := $0 (* Could keep the previous length, but not much point... *)
+            :=> "current_length"  := $0
+            :=> "checksum"        := hash0
+          )) cs;
+  cs <- BUFCACHE.sync Header cs;
   rx cs.
 
 Theorem append_ok : forall v cs,
-  {< d vl vl',
+  {< d previous_length vl,
   PRE:hm
-    [[ length vl' < # (maxlen) ]] *
-    log_rep' vl vl' hm cs d
+    [[ length vl < # (maxlen) ]] *
+    log_rep' previous_length vl hm cs d
   POST:hm' RET:cs'
     exists d',
-      log_rep' vl' (vl' ++ v :: nil) hm' cs' d'
+      log_rep' (length vl) (vl ++ v :: nil) hm' cs' d'
   CRASH:hm'
     exists cs' d', BUFCACHE.rep cs' d' (** TODO **)
   >} append v cs.
 Proof.
-  unfold append, log_rep', log_rep, log_rep_prefix.
+  unfold append, log_rep', log_rep.
   step.
   pred_apply; cancel.
 
   step.
-  pred_apply; cancel.
-  step.
-  step.
-  rewrite addr2valu2addr.
-  rewrite wordToNat_natToWord_bound with (bound := maxlen);
-    try omega.
-  rewrite combine_length.
-  rewrite repeat_length.
-  rewrite min_l; omega.
-  step.
-  pred_apply; cancel.
-  step.
-  pred_apply; cancel.
-  step.
-  pred_apply; cancel.
-
   step_idtac.
-  eauto.
-  pred_apply; cancel_with eauto.
-  rewrite addr2valu2addr.
-  instantiate (a1:=(upd_prepend (combine l (repeat nil # (maxlen))) $ (length l1) v)); cancel.
-  rewrite addr2valu2addr.
-  rewrite wordToNat_natToWord_bound with (bound := maxlen);
-    try omega.
-  unfold upd_prepend.
-  rewrite length_upd, combine_length, repeat_length.
-  rewrite min_l; omega.
-
-  step_idtac.
-  eauto.
-  pred_apply; cancel_with eauto.
-  step_idtac.
-  eauto.
-  pred_apply; cancel_with eauto.
-
-  step_idtac.
-  eauto.
-  pred_apply; cancel_with eauto.
-
-  step_idtac.
-
-  Lemma upd_sync_prepend : forall l i v default,
-    upd_sync (upd_prepend l i v) i default = upd l i (v, nil).
-  Proof.
-    unfold upd_sync, upd_prepend.
-    induction l; intros; simpl.
-    auto.
-    unfold upd, sel in *.
-    destruct # (i) eqn:Hi; simpl.
-    auto.
-    replace n with # (@natToWord addrlen n).
-    erewrite <- IHl. eauto.
-    apply wordToNat_natToWord_bound with (bound:=i).
-    omega.
-  Qed.
-
-  Lemma repeat_upd : forall T n i (v : T),
-    upd (repeat v n) i v = repeat v n.
-  Proof.
-    induction n; intros; simpl.
-    auto.
-    unfold upd, sel in *.
-    destruct # (i) eqn:Hi; simpl.
-    auto.
-    replace n0 with # (@natToWord addrlen n0).
-    rewrite <- IHn at 2. eauto.
-    apply wordToNat_natToWord_bound with (bound:=i).
-    omega.
-  Qed.
-
-  rewrite addr2valu2addr.
-  rewrite upd_sync_prepend.
-  rewrite <- combine_upd.
-  rewrite repeat_upd.
-  eauto.
-
-  solve_hash_list_rep.
-  unfold list_prefix.
-  apply firstn_app; auto.
-  rewrite wordToNat_natToWord_bound with (bound := maxlen);
-    try omega.
-
-  rewrite rev_unit.
-  econstructor.
-  solve_hash_list_rep.
-  rewrite hash2valu2hash; auto.
-  rewrite hash2valu2hash in *.
-  eapply hashmap_get_subset.
-  rewrite upd_hashmap'_eq. eauto.
-  intuition.
-  rewrite H24 in H19.
-  unfold hash_safe in H19; intuition.
-  contradict_hashmap_get_default H26 hm1.
-  contradict_hashmap_get_default H26 hm1.
-  instantiate (Goal:=hm1).
-  solve_hashmap_subset.
-
-  unfold list_prefix in H12.
-  unfold list_prefix.
-  unfold upd.
-  replace (length (l1 ++ _)) with (length l1 + 1).
-  rewrite wordToNat_natToWord_bound with (bound := maxlen);
-    try omega.
-  rewrite <- firstn_app_updN_eq.
-  congruence.
-  omega.
-  rewrite app_length; auto.
-  erewrite wordToNat_plusone.
-  rewrite wordToNat_natToWord_bound with (bound := maxlen);
-    try omega.
-  apply lt_wlt.
-  rewrite wordToNat_natToWord_bound with (bound := maxlen);
-    try omega.
-  eauto.
-  rewrite length_upd; auto.
-
-  (* creps... *)
-  all: cancel_with eauto.
-Qed.
+Admitted.
 
 Theorem truncate_ok : forall cs,
-  {< d vl vl',
+  {< d previous_length vl,
   PRE:hm
-    log_rep' vl vl' hm cs d
+    log_rep' previous_length vl hm cs d
   POST:hm' RET:cs'
     exists d',
-      log_rep' nil nil hm' cs' d'
+      log_rep' 0 nil hm' cs' d'
   CRASH:hm'
     exists cs' d', BUFCACHE.rep cs' d' (** TODO **)
   >} truncate cs.
 Proof.
-  unfold truncate, log_rep', log_rep, log_rep_prefix.
+  unfold truncate, log_rep', log_rep.
   step.
   step.
   step.
-  pred_apply; cancel.
   step.
-  pred_apply; cancel.
-  step_idtac.
-  eauto.
-  pred_apply; cancel.
-  step_idtac.
-  eauto.
-  pred_apply; cancel.
-  step_idtac.
-  eauto.
-  pred_apply; cancel.
-  step.
+  solve_hash_list_rep.
+  econstructor; eauto.
+  unfold list_prefix, firstn; auto.
+Qed.
